
\newcommand\map[3]{#1:{#2}\longrightarrow  {#3}}
\newcommand\maps[5]{{#1}:{#2}\longrightarrow {#3},{#4} \mapsto {#5}}

\aaa{Composition of lienar transformations}


Next part, we will see that the matrix multiplication interpretes the composition of linear transformations.


\a\aa














\[prop]{Let $V,W,U$ be linear spaces with bases
$$
\ce\text{ basis for }V\quad \cw\text{ basis for }W \quad \cd\text{ basis for }U
$$
Consider the following linear transformation
$$
\xymatrix{V\ar[r]^T&W\ar[r]^S&U}
$$

Then the matrix representation of $S\circ T$ is the product of matrix representations of $S$ and $T$ in corresponding bases.
}
\a\aa
We suppose the linear transformation has the following matrix representations

$$
T\underbrace{\obasis\ee n}_\ce = \underbrace{\obasis\ww m}_\cw A
$$

$$
S\underbrace{\obasis\ww m}_\cw = \underbrace{\obasis\uu p}_\cd B
$$


The proof is straightforward when looking at the commutative diagram

$$
\xymatrix{
	V\ar[rr]^T&&W\ar[rr]^S&&U\\
	\\
F^n\ar[rr]^{L_A}\ar[uu]^{L_\ce}&&F^m\ar[rr]^{L_B}\ar[uu]^{L_\cw}&&F^p\ar[uu]^{L_\cd}
	}
$$
\a\aa

\textbf{Induced transformation proof}:
$$
\xymatrix{
	V\ar[rr]^T&&W\ar[rr]^S&&U\\
	\\
F^n\ar[rr]^{L_A}\ar[uu]^{L_\ce}&&F^m\ar[rr]^{L_B}\ar[uu]^{L_\cw}&&F^p\ar[uu]^{L_\cd}
	}
$$
Let $C$ be the matrix of $S\circ T$ on the basis $\ce$ and $\cd$. We want to show $C=BA$. To do so, we only need to prove 
$$
L_C=L_B\circ L_A
$$
Since $L_C=L^{-1}_\cd\circ S\circ T\circ L_\ce$, $L_B = L_\cd^{-1}\circ S\circ L_\cw$, $L_A=L_\cw^{-1}\circ T\circ L_\ce$. Then
$$
L_B\circ L_A = L_\cd^{-1}\circ S\circ L_\cw\circ L_\cw^{-1}\circ T\circ L_\ce=L^{-1}_\cd\circ S\circ T\circ L_\ce=L_C.
$$
\a\aa

\textbf{Standard Proof:}
Since we have $$
T\underbrace{\obasis\ee n}_\ce = \underbrace{\obasis\ww m}_\cw A
$$

$$
S\underbrace{\obasis\ww m}_\cw = \underbrace{\obasis\uu p}_\cd B
$$

\[equation]{
	\[split]{
		S\circ T\underbrace{\obasis\ee n}_\ce& = S\underbrace{\obasis\ww m}_\cw A\\
		&=\underbrace{\obasis\uu p}_\cd BA
		}
	}

This implies 
$$
S\circ T\underbrace{\obasis\ee n}_\ce=\underbrace{\obasis\uu p}_\cd BA
$$
\a\aa

\[cor]{Let $V,W$ be linear spaces with bases
$$
\ce\text{ basis for }V\quad \cw\text{ basis for }W
$$
Suppose $\map TVW$ is \inve and represented by matrix $A$ on those bases, then its inverse $\map{T^{-1}}WV$ is represented by $A^{-1}$}
\a\aa
\app
By what given, we have
$$T\underbrace{\obasis\ee n}_\ce = \underbrace{\obasis\ww m}_\cw A$$
Apply $T^{-1}$ on both hand, we have
$$\underbrace{\obasis\ee n}_\ce = T^{-1}\underbrace{\obasis\ww m}_\cw A$$
Right multiplying $A^{-1}$, we have
$$\underbrace{\obasis\ee n}_\ce A^{-1}= T^{-1}\underbrace{\obasis\ww m}_\cw$$
This proves the corollary.
\ppa
\aaa



