
\newcommand\map[3]{#1:{#2}\longrightarrow  {#3}}
\newcommand\maps[5]{{#1}:{#2}\longrightarrow {#3},{#4} \mapsto {#5}}
\aaa{Left and right inverse for Linear Transformations}
We add those pages for completness, read those proofs by yourself as a homework. And try to prove it directly without using induced transformation and cancellation rule.
\a{Left Inverse for injective}
\[prop]{\RI Let $V,W$ be finite dimensional vector spaces. If $\map TVW$ is an \inj \lt, then it has a \liv $\map RWV$ with 
$$
R\circ T=\id_V
$$}
{\textbf{Proof:}Let $\ce$ be a basis of $V$, since $T$ is \inj, then $T\ce$ is also \li in $W$(By Prop.\CI). Therefore there exists a \lt $\map RWV$ with $R(T\ce)=\ce$(By Prop. \IS), therefore,
$$
R\circ T\circ L_\ce=L_\ce=\id_V\circ L_\ce
$$
Since $\ce$ \sws, $L_\ce$ is a \sur, use the \rc rule we have
$$
R\circ T=\id_V.
$$
}
\a{Right Inverse for surjective}
\[prop]{\RS Let $V,W$ be finite dimensional vector spaces. If $\map TVW$ is an \sur \lt, then it has a \riv $\map RWV$ with 
$$
T\circ R=\id_W
$$}
{\textbf{Proof:}Let $\ce$ be a basis of $V$, since $T$ is \sur, then $T\ce$ \sws $W$(By Prop.\CS). Let $\cw$ be a subtuple of $\ce$ such that $T\cw$ is a \bas of $W$. Then there exists a \lt
$
\map RWV
$
with $R(T\cw)=\cw$(By Prop \IS). So $T(R(T\cw))=T\cw$

Now we have $$T\circ R\circ L_{T\cw}=L_{T\cw}=\id_W\circ L_{T\cw}$$
Since $T\cw$ \sws, $L_{T\cw}$ is a \sur, by \rc rule we have $T\circ R=\id_W$.
}
\aaa
